Remove locking from cache
- No need to actually use busy flags for locking - can just leverage
  the Invalid cache state and the readers.
- Reader protocol is now very tight. Only addresses marked as being
  invalid (which actually means "being read filled") can have a reader,
  and readers behave exactly like a lock by the original reader.

src/ConcurrentCache.v
@@ -1,9 +1,8 @@
 Require Import CoopConcur.
 Require Import CoopConcurAuto.
 Require Import Protocols.
-Require Import Locking.
-Require Import DiskReaders.
 Require Import Star.
+Require Import DiskReaders.
 Import List.ListNotations.
 Import Hlist.HlistNotations.
 
@@ -11,31 +10,28 @@ Require Import MemCache.
 
 Section ConcurrentCache.
 
-  Definition Sigma := defState [Flags; Cache] [Locks addr; Cache; DISK].
+  (* TODO: expose Disk with readers hidden, the base of the sequential FSCQ code *)
+  Definition Sigma := defState [Cache] [Cache; DISK].
 
   (* memory variables *)
-  Definition mLocks : var (mem_types Sigma) _ := ltac:(hmember 0 (mem_types Sigma)).
-  Definition mCache : var (mem_types Sigma) _ := ltac:(hmember 1 (mem_types Sigma)).
+  Definition mCache : var (mem_types Sigma) _ := ltac:(hmember 0 (mem_types Sigma)).
 
   (* abstraction ("virtual") variables *)
-  Definition vLocks : var (abstraction_types Sigma) _
-    := ltac:(hmember 0 (abstraction_types Sigma)).
   Definition vCache : var (abstraction_types Sigma) _
-    := ltac:(hmember 1 (abstraction_types Sigma)).
+    := ltac:(hmember 0 (abstraction_types Sigma)).
   Definition vDisk : var (abstraction_types Sigma) _
-    := ltac:(hmember 2 (abstraction_types Sigma)).
+    := ltac:(hmember 1 (abstraction_types Sigma)).
 
   Definition cacheR (tid:TID) : Relation Sigma :=
     fun s s' =>
       let ld := get vDisk s in
       let ld' := get vDisk s' in
-      let locks := get vLocks s in
-      let locks' := get vLocks s' in
       same_domain ld ld' /\
-      (* lock protects virtual disk *)
-      (forall a, locks a = Owned tid ->
-            ld' a = ld a) /\
-      lock_protocol tid locks locks'.
+      (* a locking-like protocol, but true for any provable program
+      due to the program semantics themselves *)
+      (forall a v tid', ld a = Some (v, Some tid') ->
+                   tid <> tid' ->
+                   ld' a = Some (v, Some tid')).
 
   Definition addr_lock (l:Flags) (a:addr) :=
     get_lock l #a.
@@ -43,21 +39,18 @@ Section ConcurrentCache.
   Definition cacheI : Invariant Sigma :=
     fun d m s =>
       get mCache m = get vCache s /\
-      locks_rep (addr_lock (get mLocks m)) (get vLocks s) /\
       cache_rep d (get vCache s) (get vDisk s).
 
-  Hint Resolve same_domain_refl.
+  Hint Resolve same_domain_refl same_domain_trans.
   Hint Resolve lock_protocol_refl.
 
   Theorem cacheR_trans_closed : forall tid s s',
       star (cacheR tid) s s' ->
       cacheR tid s s'.
   Proof.
-    intros.
-    apply trans_closed; auto; intuition.
-    unfold cacheR; intuition.
-    admit.
-  Admitted.
+    intro tid.
+    apply trans_closed; unfold cacheR; intuition eauto.
+  Qed.
 
   Definition delta : Protocol Sigma :=
     defProtocol cacheI cacheR cacheR_trans_closed.
@@ -66,55 +59,39 @@ Section ConcurrentCache.
     c <- Get mCache;
       rx (cache_val c a).
 
+  Definition modify_cache {T} (up: Cache -> Cache) rx : prog Sigma T :=
+    c <- Get mCache;
+      _ <- Assgn mCache (up c);
+      _ <- var_update vCache up;
+      rx tt.
+
   Definition cache_write {T} a v rx : prog Sigma T :=
     tid <- GetTID;
-    c <- Get mCache;
-      let c' := cache_add c a (Dirty v) in
-      _ <- Assgn mCache c';
-        _ <- var_update vCache
-          (* fix cache *)
-          (fun c => cache_add c a (Dirty v));
-        _ <- var_update vDisk
-          (* update virtual disk *)
-          (fun vd => upd vd a (v, Some tid));
-        rx tt.
+      (* may fill an invalid entry - filling thread will notice this
+      and keep the new value *)
+      _ <- modify_cache (fun c => cache_add c a (Dirty v));
+      _ <- var_update vDisk
+        (* update virtual disk *)
+        (fun vd => upd vd a (v, Some tid));
+      rx tt.
 
   Definition AsyncRead {T} a rx : prog Sigma T :=
     tid <- GetTID;
-      _ <- StartRead a;
+      _ <- StartRead_upd a;
       _ <- var_update vDisk
         (fun vd => add_reader vd a tid);
       _ <- Yield a;
-      v <- FinishRead a;
+      v <- FinishRead_upd a;
       _ <- var_update vDisk
         (fun vd => remove_reader vd a);
       rx v.
 
-  Definition lock {T} (a: addr) rx : prog Sigma T :=
-    tid <- GetTID;
-      _ <- wait_for mLocks (is_open #a) a;
-      l <- Get mLocks;
-      _ <- Assgn mLocks (set_locked l #a);
-      _ <- var_update vLocks
-        (fun l => upd_lock l a (Owned tid));
-      rx tt.
-
-  Definition unlock {T} (a: addr) rx : prog Sigma T :=
-    l <- Get mLocks;
-      _ <- Assgn mLocks (free_lock l #a);
-      _ <- var_update vLocks
-        (fun l => upd_lock l a NoOwner);
-      rx tt.
-
   Definition cache_fill {T} a rx : prog Sigma T :=
-    _ <- lock a;
+    _ <- modify_cache (fun c => cache_invalidate c a);
       v <- AsyncRead a;
-      c <- Get mCache;
-      let c' := cache_add c a (Clean v) in
-      _ <- Assgn mCache c';
-        _ <- var_update vCache
-          (fun c => cache_add c a (Clean v));
-        _ <- unlock a;
-        rx tt.
+      _ <- modify_cache (fun c => cache_add c a (Clean v));
+      _ <- var_update vCache
+        (fun c => cache_add c a (Clean v));
+      rx tt.
 
 End ConcurrentCache.
